theories/micromega/QMicromega.v
@@ -153,8 +153,8 @@ Proof.
   - apply Qlt_bool_iff.
 Qed.
 
-Definition Qeval_op2 (k:kind) :  Op2 ->  Q -> Q -> Tauto.rtyp k:=
-  if k as k0 return (Op2 -> Q -> Q -> Tauto.rtyp k0)
+Definition Qeval_op2 (k:kind) :  Op2 ->  Q -> Q -> eKind k:=
+  if k as k0 return (Op2 -> Q -> Q -> eKind k0)
   then Qeval_pop2 else Qeval_bop2.
 
 
